automation

tools/coq2latex/coq2latex/CoqParsing.cs
@@ -1,0 +1,152 @@
+﻿using System;
+using System.Collections.Generic;
+using System.Diagnostics;
+using System.Linq;
+using System.Text;
+using System.Text.RegularExpressions;
+using System.Threading.Tasks;
+
+namespace coq2latex
+{
+    class CoqParsing
+    {
+        public static readonly string regexCoqExpression =
+            @"\s*?" +
+            @"(\(((?<BR>\()|(?<-BR>\))|[^()]*)+\)(?(BR)(?!))" +
+            @"|(\w|\'|\\)+)" +
+            @"\s*?";
+
+        private string coqFile;
+        public Dictionary<string, Tuple<int, Func<string[], string>>> latexifyExpression;
+
+        public CoqParsing(string coqFile)
+        {
+            this.coqFile = coqFile;
+            this.latexifyExpression = new Dictionary<string, Tuple<int, Func<string[], string>>>();
+        }
+
+        public string LatexifyExpression(string coq)
+        {
+            coq.Replace("[]", @"\emptyset");
+            coq.Replace("::", @"*");
+            coq = coq.Trim();
+            if (coq == "")
+                return coq;
+            if (!Regex.IsMatch(coq, "^(" + regexCoqExpression + ")+$"))
+            {
+                var sparseMatches = Regex.Matches(coq, regexCoqExpression).OfType<Match>().Reverse();
+                var coqX = coq;
+                // erase expressions
+                foreach (var match in sparseMatches)
+                    coqX = coqX.Remove(match.Index, match.Length).Insert(match.Index, new string(' ', match.Length));
+                // get delimiters
+                var delims = new List<Tuple<int, int>>();
+                while (coqX.Trim() != "")
+                {
+                    coqX = coqX.TrimEnd();
+                    var index2 = coqX.Length;
+                    var index1 = coqX.LastIndexOf(' ') + 1;
+                    delims.Add(new Tuple<int, int>(index1, index2));
+                    coqX = coqX.Substring(0, index1);
+                }
+                delims.Add(new Tuple<int, int>(0, 0));
+                // replace
+                var lastDelimStart = coq.Length;
+                foreach (var delim in delims)
+                {
+                    var part = coq.Substring(delim.Item2, lastDelimStart - delim.Item2);
+                    part = " " + LatexifyExpression(part) + " ";
+                    coq = coq.Remove(delim.Item2, lastDelimStart - delim.Item2).Insert(delim.Item2, part);
+                    lastDelimStart = delim.Item1;
+                }
+
+                return coq;
+                // special handlers:
+                // - A = B
+                if (coqX.Count(c => c == '=') == 1)
+                {
+                    int index = coqX.IndexOf('=');
+                    return
+                        LatexifyExpression(coq.Substring(0, index)) +
+                        " = " +
+                        LatexifyExpression(coq.Substring(index + 1));
+                }
+                // - anything else
+                var indices = coqX.Select((x, i) => new { X = x, I = i }).Where(x => x.X == ',').Select(x => x.I).ToList();
+                indices.Reverse();
+                indices.Add(-1);
+                var lastIndex = coq.Length;
+                foreach (var index in indices)
+                {
+                    string part = coq.Substring(index + 1, lastIndex - index - 1);
+                    coq = coq.Remove(index + 1, lastIndex - index - 1).Insert(index + 1, " " + LatexifyExpression(part));
+                    lastIndex = index;
+                }
+                return coq.Trim();
+
+                return @"\verb€" + coq + "€";
+            }
+            var matches = Regex.Matches(coq, regexCoqExpression);
+            if (matches.Count == 1)
+                if (coq.StartsWith("("))
+                {
+                    var inner = LatexifyExpression(coq.Substring(1, coq.Length - 2));
+                    if (inner.Contains(" "))
+                        return "(" + inner + ")";
+                    else
+                        return inner;
+                }
+                else
+                {
+                    if (latexifyExpression.ContainsKey(coq))
+                    {
+                        var handler = latexifyExpression[coq];
+                        if (handler.Item1 == 0)
+                            return handler.Item2(new string[0]);
+                    }
+                    return coq;
+                }
+            var xs = matches.OfType<Match>().Select(x => x.Value).Select(LatexifyExpression);
+            if (latexifyExpression.ContainsKey(xs.First()))
+            {
+                var handler = latexifyExpression[xs.First()];
+                if (handler.Item1 == matches.Count - 1)
+                    return handler.Item2(xs.Skip(1).ToArray());
+            }
+            return string.Join(" ", xs);
+        }
+
+        public IEnumerable<string> ParseInductive(string name)
+        {
+            Debug.WriteLine("Inductive: " + name);
+            Regex regex = new Regex("Inductive " + name + ".*?:=(?<def>.*?)\\.",
+                RegexOptions.ExplicitCapture |
+                RegexOptions.Singleline);
+            var match = regex.Match(coqFile);
+            var s = match.Groups["def"].Value;
+
+            Regex regexCtor = new Regex(@"\|(?<name>.*?):.*?,(?<pre>([^|]*?->)*)(?<con>.*?)(?=$|\|)",
+                RegexOptions.ExplicitCapture |
+                RegexOptions.Singleline);
+            foreach (Match ctor in regexCtor.Matches(s))
+            {
+                var cname = ctor.Groups["name"].Value.Trim();
+                var ccon = ctor.Groups["con"].Value.Trim();
+                var cprems = ctor.Groups["pre"].Value.Split(new string[] { "->" }, StringSplitOptions.RemoveEmptyEntries).Select(x => x.Trim()).ToArray();
+
+                Debug.WriteLine("\tCtor: " + cname);
+
+                StringBuilder res = new StringBuilder();
+                res.AppendLine(@"\begin{mathpar}");
+                res.AppendLine(@"\inferrule* [right=" + cname + "]");
+                if (cprems.Length == 0)
+                    res.AppendLine("{~}");
+                else
+                    res.AppendLine("{" + string.Join(@" \\ ", cprems.Select(LatexifyExpression)) + "}");
+                res.AppendLine("{" + LatexifyExpression(ccon) + "}");
+                res.AppendLine(@"\end{mathpar}\hfill");
+                yield return res.ToString();
+            }
+        }
+    }
+}
