tools/coq2latex/coq2latex/Program.cs
@@ -1,7 +1,10 @@
 ﻿using System;
 using System.Collections.Generic;
+using System.Diagnostics;
+using System.IO;
 using System.Linq;
 using System.Text;
+using System.Text.RegularExpressions;
 using System.Threading.Tasks;
 
 namespace coq2latex
@@ -10,7 +13,137 @@ namespace coq2latex
     {
         static void Main(string[] args)
         {
+            Debug.Listeners.Add(new ConsoleTraceListener());
 
+            string coqFileName = "GradVer.v";
+            string coqFile;
+            DirectoryInfo dir = new DirectoryInfo(Directory.GetCurrentDirectory());
+            while (dir != null && !dir.EnumerateFiles(coqFileName).Any())
+                dir = dir.Parent;
+            if (dir == null)
+                throw new FileNotFoundException(coqFileName);
+            coqFile = File.ReadAllText(dir.FullName + "\\" + coqFileName);
+            var parsing = new CoqParsing(coqFile);
+            var le = parsing.latexifyExpression;
+
+            // coq aliases
+            string staticExpression = "sfrme";
+            string staticFormula = "sfrmphi'";
+            string staticSemantics = "hoareSingle";
+
+            Action<string, string> commandify2 = (s, t) => le[s] = new Tuple<int, Func<string[], string>>(0, _ => @"\" + t);
+            Action<string> commandify = s => commandify2(s, s);
+            Action<string> swallowCtor = s => le[s] = new Tuple<int, Func<string[], string>>(1, x => x[0]);
+            Action<string, string> functionify2 = (s, t) => le[s] = new Tuple<int, Func<string[], string>>(1, x => @"\" + t + "(" + x[0] + ")");
+            Action<string> functionify = s => functionify2(s, s);
+
+            le[staticExpression] = new Tuple<int, Func<string[], string>>(
+                2,
+                x => x[0] + @" \sfrme " + x[1]
+            );
+            le[staticFormula] = new Tuple<int, Func<string[], string>>(
+                2,
+                x => x[0] + @" \sfrmphi " + x[1]
+            );
+            le["sfrmphi"] = new Tuple<int, Func<string[], string>>(
+                2,
+                x => x[0] + @" \sfrmphi " + x[1]
+            );
+            le[staticSemantics] = new Tuple<int, Func<string[], string>>(
+                4,
+                x => @"\hoare {" + x[0] + "} {" + x[1] + "} {" + x[2] + "} {" + x[3] + "}"
+            );
+            le["In"] = new Tuple<int, Func<string[], string>>(
+                2,
+                x => x[0] + @" \in " + x[1]
+            );
+            swallowCtor("ev");
+            swallowCtor("ex");
+            le["edot"] = new Tuple<int, Func<string[], string>>(
+                2,
+                x => x[0] + "." + x[1]
+            );
+            le["appEnd"] = new Tuple<int, Func<string[], string>>(
+                2,
+                x => x[0] + @"{\:*\:}" + x[1]
+            );
+            commandify2("phiTrue", "true");
+            le["phiEq"] = new Tuple<int, Func<string[], string>>(
+                2,
+                x => x[0] + @"{\:=\:}" + x[1]
+            );
+            le["phiImplies"] = new Tuple<int, Func<string[], string>>(
+                2,
+                x => x[0] + @"{\:\implies\:}" + x[1]
+            );
+            le["phiNeq"] = new Tuple<int, Func<string[], string>>(
+                2,
+                x => x[0] + @"{\:\neq\:}" + x[1]
+            );
+            le["phiAcc"] = new Tuple<int, Func<string[], string>>(
+                2,
+                x => @"\acc(" + x[0] + "," + x[1] + ")"
+            );
+            le["phiSubst"] = new Tuple<int, Func<string[], string>>(
+                3,
+                x => x[2] + "[" + x[0] + "/" + x[1] + "]"
+            );
+            le["sAlloc"] = new Tuple<int, Func<string[], string>>(
+                2,
+                x => x[0] + @"{\::=\:\new\:}" + x[1]
+            );
+            le["sMemberSet"] = new Tuple<int, Func<string[], string>>(
+                3,
+                x => x[0] + @"{\::=\:}" + x[1] + "." + x[2]
+            );
+            le["sAssign"] = new Tuple<int, Func<string[], string>>(
+                3,
+                x => x[0] + @"{\::=\:}" + x[1]
+            );
+            le["sReturn"] = new Tuple<int, Func<string[], string>>(
+                1,
+                x => @"{\return}" + x[0]
+            );
+            le["sAssert"] = new Tuple<int, Func<string[], string>>(
+                1,
+                x => @"{\assert}" + x[0]
+            );
+            le["sRelease"] = new Tuple<int, Func<string[], string>>(
+                1,
+                x => @"{\release}" + x[0]
+            );
+            functionify("Gamma");
+            functionify("rho");
+            functionify2("fieldsNames", "fields");
+
+            swallowCtor("Some");
+            swallowCtor("TClass");
+            commandify2("TPrimitiveInt", "Tint");
+            commandify("vnull");
+            commandify("xresult");
+            commandify("xthis");
+
+            le["fold_left"] = new Tuple<int, Func<string[], string>>(
+                3,
+                x =>
+                {
+                    var funMatch = Regex.Match(x[0], @"^\(\s*fun\s+(?<a1>.*?)\s+(?<a2>.*?)\s*=>(?<body>.*)\)$", RegexOptions.Singleline);
+                    var funBody = funMatch.Groups["body"].Value;
+                    funBody = funBody.Replace(funMatch.Groups["a2"].Value, x[1]);
+                    funBody = funBody.Replace(funMatch.Groups["a1"].Value, x[2]);
+                    return @"\overline{" + funBody + "}";
+                }
+            );
+
+            File.WriteAllLines(dir.FullName + "\\latex\\staticExpression.tex",
+                parsing.ParseInductive(staticExpression));
+            File.WriteAllLines(dir.FullName + "\\latex\\staticFormula.tex",
+                parsing.ParseInductive(staticFormula));
+            File.WriteAllLines(dir.FullName + "\\latex\\staticSemantics.tex",
+                parsing.ParseInductive(staticSemantics));
+
+            Console.WriteLine("DONE");
+            //Console.ReadKey();
         }
     }
 }
